Core/Eval/Soundness.lean
@@ -1,20 +1,80 @@
 import LeanSubst
 import Core.Reduction
+import Core.Reduction.Definition
 import Core.Eval.SmallStep
 
+open Lilac
 
 namespace Core
 
+theorem Term.is_data_sound :
+  Term.is_data dc s = some c ->
+  Term.IsData dc s c
+:= by
+  intro h
+  fun_induction Term.is_data <;> simp at *
+  case _ =>
+    subst h; apply Term.IsData.nil
+  case _ ih =>
+    rw[Option.bind_eq_some_iff] at h; rcases h with ⟨h1, h2, h⟩
+    simp at h; rcases h with ⟨h3, h4⟩
+    subst c; subst dc
+    replace ih := ih h2
+    apply Term.IsData.cons
+    apply ih
+    simp; apply And.intro
+    · rfl
+    · apply And.intro
+      · rfl
+      · apply And.intro
+        · rfl
+        · apply And.intro
+          · rfl
+          · apply And.intro
+            · rfl
+            · apply And.intro
+              · rfl
+              · rfl
+    rfl
+
+
+theorem get_instance_sound {G : List Global} :
+   get_instance x cs G = some ⟨i, _, p, t⟩ ->
+   G[i]? = some (Global.inst x p t)
+:= by
+intro h
+induction G <;> (unfold get_instance at h; unfold get_instance_aux at h; simp at *)
+sorry
+
+theorem pattern_match_sound {m : Nat} {cs : Vec Constructor m} {ps : Pattern m} :
+  pattern_match cs ps = true ->
+  Core.Pattern.Match cs ps
+:= by
+
+sorry
+
 theorem eval_sound (Γ : GlobalEnv) :
-  eval Γ M = some N ->
+  M.eval Γ = some N ->
   Γ ⊢ M ~> N := by
 intro h
-fun_induction eval <;> simp at h
+fun_induction Term.eval <;> simp at h
 case _ =>  -- lookup defn
-  sorry
-
-case _ => -- openm
-  sorry
+  rw[Option.bind_eq_some_iff] at h; rcases h with ⟨h1, h2, h⟩
+  cases h;
+  apply Red.defn h2
+case _ ih => -- openm
+  rw[Option.bind_eq_some_iff] at h; rcases h with ⟨h1, h2, h⟩
+  rw[Option.bind_eq_some_iff] at h; rcases h with ⟨⟨i, m, p, t⟩, h4, h⟩
+  simp at h; rcases h with ⟨⟨e1, h5⟩, h⟩
+  subst e1;
+  replace h2 := Term.is_data_sound h2
+  replace h4 := get_instance_sound h4
+  replace h5 := pattern_match_sound (cs := h1) (ps := p) h5
+  apply Red.openm_match (i := i) (b := t) (b' := N)
+  · apply h2
+  · apply h4
+  · apply h5
+  · simp; symm at h; apply h
 
 case _ => -- openm
   sorry
@@ -49,6 +109,18 @@ case _ =>
 case _ =>
   sorry
 
+case _ =>
+  sorry
+case _ =>
+  sorry
+
+case _ =>
+  sorry
+case _ =>
+  sorry
+
+case _ =>
+  sorry
 case _ =>
   sorry
 
