Core/Examples/TypeFunction.lean
@@ -17,7 +17,6 @@ def mkApps (d : Term) (tys : List Ty) (ts : List Term) : Term :=
 end Core.Term
 
 namespace Core.Ty
-
 def mkApps (d : Ty) (tys : List Ty) : Ty :=
   List.foldl (λ f a => f • a ) d tys
 end Core.Ty
@@ -33,21 +32,21 @@ def TypeFunCtx : GlobalEnv := [
   --     let j : (a' ~ a'') = (h1 ; sym k1).2
   --     let e1' : F a'' b' = e1 ▹ <F> `@c[ j ] `@c[<b'>]
   --       sym h2 ; <Maybe> `@c fdF[a''][b'][b''] e1' e2 ; k2
-  -- .inst "fdF" #(⟨"FMM", 2, #(t#2, t#1), 2, 3⟩, ⟨"FMM", 2, #(t#2, t#0), 2, 3⟩)
-  --       (let sk1 := Term.mkApps d#"sym" [gt#"Maybe" • t#1, t#6] [#2]
-  --       let t := Term.mkApps d#"seq" [gt#"Maybe" • t#3, t#6, gt#"Maybe" • t#1] [#5, sk1]
-  --       let j := prj[1] t
-  --       -- let j : (a' ~ a'') = (h1 ; sym k1).2
-  --       let sh2 := Term.mkApps d#"sym" [gt#"Maybe" • t#2, t#5] [#4]
-  --       let e1' := Term.cast t#0
-  --                   ((d#"appc2").mkApps [gt#"F", gt#"F", t#3, t#1, t#2, t#2] [refl! gt#"F", j, refl! t#2])
-  --                   #3
-  --       -- let e1' : F a'' b' = e1 ▹ <F> `@c[ j ] `@c[<b'>]
-  --       let e3 := (d#"appc").mkApps [gt#"Maybe", gt#"Maybe", t#2, t#0] [(refl! gt#"Maybe"), (openm! "fdF" #(t#1, t#2, t#0) #() #(e1', #0).to)]
-  --       -- let e3 : Maybe b' ~ Maybe b'' = <Maybe> `@c fdF[a''][b'][b''] e1' e2
-  --       (d#"seq").mkApps [t#5, gt#"Maybe" • t#2, t#4]
-  --                 [sh2, (d#"seq").mkApps [gt#"Maybe" • t#2, gt#"Maybe" • t#0, t#4] [e3, #1]]),
-  --        -- sym h2 ; e3 ; k2
+  .inst "fdF" #(⟨"FMM", 2, #(t#2, t#1), 2, 3⟩, ⟨"FMM", 2, #(t#2, t#0), 2, 3⟩)
+        (let sk1 := Term.mkApps d#"sym" [gt#"Maybe" • t#1, t#6] [#2]
+        let t := Term.mkApps d#"seq" [gt#"Maybe" • t#3, t#6, gt#"Maybe" • t#1] [#5, sk1]
+        let j := prj[1] t
+        -- let j : (a' ~ a'') = (h1 ; sym k1).2
+        let sh2 := Term.mkApps d#"sym" [gt#"Maybe" • t#2, t#5] [#4]
+        let e1' := Term.cast t#0
+                    ((d#"appc2").mkApps [gt#"F", gt#"F", t#3, t#1, t#2, t#2] [refl! gt#"F", j, refl! t#2])
+                    #3
+        -- let e1' : F a'' b' = e1 ▹ <F> `@c[ j ] `@c[<b'>]
+        let e3 := (d#"appc").mkApps [gt#"Maybe", gt#"Maybe", t#2, t#0] [(refl! gt#"Maybe"), (openm! "fdF" #(t#1, t#2, t#0) #() #(e1', #0).to)]
+        -- let e3 : Maybe b' ~ Maybe b'' = <Maybe> `@c fdF[a''][b'][b''] e1' e2
+        (d#"seq").mkApps [t#5, gt#"Maybe" • t#2, t#4]
+                  [sh2, (d#"seq").mkApps [gt#"Maybe" • t#2, gt#"Maybe" • t#0, t#4] [e3, #1]]),
+         -- sym h2 ; e3 ; k2
 
 
   -- FMM : ∀ a b a' b'. Maybe a' ~ a → Maybe b' ~ b → F a' b' → F a b
@@ -79,6 +78,19 @@ def TypeFunCtx : GlobalEnv := [
 
 #guard TypeFunCtx.wf_globals == some ()
 #guard GlobalEnv.check_open_exhaustive TypeFunCtx == none
+
+
+-- f : ∀ t. F Int t → t → t
+--   = Λ t λ (d : F Int t).
+--     let h : Bool ~ t = fdF[Int][Bool][t](FIB [Int][Bool] <Int> <Bool>) d in
+--     not ▹ <→> `@c h `@c h
+def fnot := Λ[★]λ[(gt#"F" • gt#"Int") • t#0]λ[t#0]
+            let iFIB := inst! "FIB" #(gt#"Int", gt#"Bool") #() (#(refl! gt#"Int", refl! gt#"Bool").to)
+            let h := openm! "fdF" #(gt#"Int", gt#"Bool", t#0) #() #(iFIB, #1).to
+            (Term.cast t#0 ((d#"arrowc").mkApps [gt#"Bool", t#0, gt#"Bool", t#0] [h, h]) notTerm) • #0
+
+#eval! fnot.infer_type TypeFunCtx [] []
+
 
   --   Λ t u v. λ d1 d2.
   --     If FMM[t][u] ← d1 then Λ a' b'. λ (h1: Maybe a' ~  t) (h2 : Maybe b' ~ u) (e1 : F a' b').
@@ -145,10 +157,10 @@ some ([★, ★, ★, ★, ★, ★, ★],
   --         3, #((gt#"Maybe" • t#1) ~[★]~ t#3, (gt#"Maybe" • t#0) ~[★]~ t#2, (gt#"F" • t#1) • t#0),
   --            ((gt#"F" • t#3) • t#2)⟩,
 
-#eval!
-  pattern_binders TypeFunCtx
-    [★, ★, ★] 2 #( ((gt#"F" • t#2) • t#1), ((gt#"F" • t#2) • t#0))
-    #(⟨"FMM", 2, #(t#2, t#1), 2, 3⟩, ⟨"FMM", 2, #(t#2, t#0), 2, 3⟩)
+-- #eval!
+--   pattern_binders TypeFunCtx
+--     [★, ★, ★] 2 #( ((gt#"F" • t#2) • t#1), ((gt#"F" • t#2) • t#0))
+--     #(⟨"FMM", 2, #(t#2, t#1), 2, 3⟩, ⟨"FMM", 2, #(t#2, t#0), 2, 3⟩)
 
 --some ([], [gt#F • t#3 • t#2, gt#F • t#2 • t#1, gt#F • t#4 • t#3, gt#F • t#4 • t#3])
 -- #eval!
@@ -184,16 +196,5 @@ some ([★, ★, ★, ★],
 --       else none
 --   | _ => none
 
-
--- f : ∀ t. F Int t → t → t
---   = Λ t λ (d : F Int t).
---     let h : Bool ~ t = fdF[Int][Bool][t](FIB [Int][Bool] <Int> <Bool>) d in
---     not ▹ <→> `@c h `@c h
-def fnot := Λ[★]λ[(gt#"F" • gt#"Int") • t#0]λ[t#0]
-            let iFIB := inst! "FIB" #(gt#"Int", gt#"Bool") #() (#(refl! gt#"Int", refl! gt#"Bool").to)
-            let h := openm! "fdF" #(gt#"Int", gt#"Bool", t#0) #() #(iFIB, #1).to
-            (Term.cast t#0 ((d#"arrowc").mkApps [gt#"Bool", t#0, gt#"Bool", t#0] [h, h]) notTerm) • #0
-
-#eval! fnot.infer_type TypeFunCtx [] []
 
 end Core.Examples
